
$$
\vec{L_{0}} =  m \vec{OM} \wedge \overrightarrow{x}
$$

$$
\overrightarrow{L_{O}} = m \overrightarrow{OM} \wedge \overrightarrow{v} = mR^{2}\dot{\theta}\overrightarrow{u_{z}}

$$

$$
\overrightarrow{\mathcal{M}_{0}}(\overrightarrow{f}) = \overrightarrow{OM} \wedge \overrightarrow{f}

\mathcal{M}_{\Delta}(\overrightarrow{f}) = \overrightarrow{\mathcal{M}_{0}}(\overrightarrow{f}) \cdot  \overrightarrow{u_{\Delta}} = (\overrightarrow{OM} \wedge \overrightarrow{f}) \cdot  \overrightarrow{u_{\Delta}}
$$


$$
\frac{d \overrightarrow{L_{O}}}{dt}  = \sum_{i} \overrightarrow{\mathcal{M}_{0}}(\overrightarrow{f_{i}})
$$


$$
f_{r} = - \frac{dE_{p}}{dt}
$$


$$
\vec{f} = - \mathscr{G} \frac{m_{1} m_{2}}{r^{2}} \vec{u_{r}}
$$

$$
\frac{dE_{p}}{dr} =  \mathscr{G} \frac{m_{1} m_{2}}{r^{2}}  = \frac{d}{dr} \left( - \mathscr{G} \frac{m_{1} m_{2}}{r} \right) \implies \boxed {  \overrightarrow{E_{p}} = - \mathscr{G} \frac{m_{1} m_{2}}{r}}
$$

$$
\vec{f} = - \frac{1}{4 \pi \varepsilon_{0}} \frac{q_{1} q_{2}}{r^{2}} \vec{u_{r}}
$$

$$
\frac{dE_{p}}{dr} = - \frac{1}{4 \pi \varepsilon_{0}} \frac{q_{1} q_{2}}{r^{2}} = \frac{d}{dr} \left( \frac{1}{4 \pi \varepsilon_{0}} \frac{q_{1} q_{2}}{r}\right)  \implies \boxed{ E_{p} =  \frac{q_{1} q_{2}}{4 \pi \varepsilon_{0}r} }
$$

$$
\vec{f} = -\frac{K}{r^{2}}\overrightarrow{u_{r}}
$$

$$
E_{p}(r) = -\frac{K}{r}
$$

$$
\mathscr{C} = r^{2}\dot{\theta} = \frac{\|\overrightarrow{L_{0}}\|}{m}
$$


$$
\Delta \mathscr{A} = \frac{\mathscr{C}}{2}\Delta t

[ \! [ 1, n] \!]


$$


$$
U = \frac{1}{2} k a^{2} + \mathscr{C}
$$

$$
\underset{ M_{1} \to M_{2} }{ \Delta E_{m} } = \underset{  M_{1} \underset{ \mathscr{C} }{ \to } M_{2}  }{ W_{nc} }
$$
